defined arithmetic hierarchy

Computability/Jump.lean
@@ -13,17 +13,30 @@ state the jump theorems:
 -/
 
 /-
-A set A is recursively enumerable in a family of partial recursive functions g if its characteristic
-function is recursive in the family g.
+A set A is recursively enumerable in a set of partial recursive functions `O` if its characteristic
+function is recursive in `O`.
 -/
-def recursively_enumerable_in (g : α → ℕ →. ℕ) (A : ℕ → Prop) :=
-  ∃ f, (RecursiveIn (Set.range g) f) ∧ (∀ n, A n ↔ n ∈ f.Dom)
+def recursively_enumerable_in (O : Set (ℕ →. ℕ)) (A : Set ℕ) :=
+  ∃ f, (RecursiveIn O f) ∧ A = f.Dom
+
+/-
+A set A is recursively enumerable in a family of partial recursive functions `X` if its characteristic
+function is recursive in `X`.
+-/
+def recursively_enumerable_in₁ (X : α → ℕ →. ℕ) (A : Set ℕ) :=
+  ∃ f, (RecursiveIn (Set.range X) f) ∧ A = f.Dom
 
 /-
 A set A is re in a single partial recursive function g if its characteristic function is recursive in g.
 -/
-def recursively_enumerable_in₁ (g : ℕ →. ℕ) (A : ℕ → Prop) :=
-  ∃ f, (RecursiveIn {g} f) ∧ (∀ n, A n ↔ n ∈ f.Dom)
+def recursively_enumerable_in₂ (g : ℕ →. ℕ) (A : ℕ → Prop) :=
+ ∃ f, (RecursiveIn {g} f) ∧ A = f.Dom
+
+/-
+A set A is recursively enumerable if its characteristic function is recursive in the empty set.
+-/
+def recursively_enumerable (A : Set ℕ) :=
+  ∃ f, (RecursiveIn {} f) ∧ A = f.Dom
 
 /-
 The jump of f is the diagonal of the universal machine relative to f:
@@ -67,14 +80,14 @@ theorem jump_recIn (f : ℕ →. ℕ) : f ≤ᵀ (f⌜) := by sorry
 theorem jump_not_reducible (f : ℕ →. ℕ) : ¬(f⌜ ≤ᵀ f) := by sorry
 
 theorem re_iff_one_one_jump  (A : Set ℕ) (f : ℕ →. ℕ) :
-recursively_enumerable_in₁ f A ↔ OneOneReducible A (f⌜).Dom := by sorry
+recursively_enumerable_in₂ f A ↔ OneOneReducible A (f⌜).Dom := by sorry
 
 theorem re_in_trans (A : Set ℕ) (f h : ℕ →. ℕ) :
-  recursively_enumerable_in₁ f A →
+  recursively_enumerable_in₂ f A →
   f ≤ᵀ h →
-  recursively_enumerable_in₁ h A := by
+  recursively_enumerable_in₂ h A := by
   intro freInA fh
-  simp [recursively_enumerable_in₁] at *
+  simp [recursively_enumerable_in₂] at *
   obtain ⟨g, hg, hA⟩ := freInA
   use g
   constructor
